backend/ValueAnalysis.v
@@ -2058,6 +2058,187 @@ Proof.
   - intros. inv H0. inv H. constructor; eauto.
 Qed.
 
+(** ** Block classification for an injection *)
+
+Program Definition bc_of_inj (f: meminj) (se: Genv.symtbl) :=
+  {|
+    bc_img b :=
+      if f b then
+        match Genv.invert_symbol se b with
+        | Some id => BCglob id
+        | None => BCother
+        end
+      else
+        BCinvalid
+  |}.
+Next Obligation.
+  destruct (f b1); try discriminate.
+  destruct Genv.invert_symbol; discriminate.
+Qed.
+Next Obligation.
+  destruct (f b1); try discriminate.
+  destruct (f b2); try discriminate.
+  destruct (Genv.invert_symbol se b1) eqn:Hb1; inv H.
+  destruct (Genv.invert_symbol se b2) eqn:Hb2; inv H0.
+  apply Genv.invert_find_symbol in Hb1.
+  apply Genv.invert_find_symbol in Hb2.
+  congruence.
+Qed.
+
+Lemma bc_of_symtbl_inj f se1 se2:
+  Genv.match_stbls f se1 se2 ->
+  bc_incr (bc_of_symtbl se1) (bc_of_inj f se1).
+Proof.
+  intros Hse b Hb. cbn in *.
+  destruct Genv.invert_symbol eqn:H; try congruence.
+  apply Genv.invert_find_symbol in H.
+  edestruct @Genv.find_symbol_match as (tb & Htb & _); eauto.
+  rewrite Htb. auto.
+Qed.
+
+Lemma bc_of_symtbl_inj_glob f se b id:
+  bc_of_inj f se b = BCglob id ->
+  bc_of_symtbl se b = BCglob id.
+Proof.
+  unfold bc_of_inj, bc_of_symtbl; cbn.
+  destruct f; try discriminate.
+  destruct Genv.invert_symbol; congruence.
+Qed.
+
+Lemma bc_of_inj_genv_match f se1 se2:
+  Genv.match_stbls f se1 se2 ->
+  genv_match (bc_of_inj f se1) se1.
+Proof.
+  intros Hse. split.
+  - intros id b1. split.
+    + intros Hb1.
+      edestruct @Genv.find_symbol_match as (b2 & Hb12 & Hb2); eauto.
+      apply Genv.find_invert_symbol in Hb1. cbn.
+      rewrite Hb12, Hb1. auto.
+    + cbn.
+      destruct (f b1) eqn:Hb; try discriminate.
+      destruct Genv.invert_symbol eqn:Hid; try discriminate.
+      intro. apply Genv.invert_find_symbol. congruence.
+  - intros b1 Hb1. cbn.
+    eapply Genv.mge_dom in Hb1 as [b2 Hb]; eauto. rewrite Hb.
+    destruct Genv.invert_symbol; split; discriminate.
+Qed.
+
+Lemma bc_of_inj_pmatch f se1 b1 ofs1 v2:
+  Val.inject f (Vptr b1 ofs1) v2 ->
+  pmatch (bc_of_inj f se1) b1 ofs1 Ptop.
+Proof.
+  inversion 1; subst.
+  constructor. cbn.
+  rewrite H2.
+  destruct Genv.invert_symbol; discriminate.
+Qed.
+
+Lemma bc_of_inj_vmatch f se1 v1 v2:
+  Val.inject f v1 v2 ->
+  vmatch (bc_of_inj f se1) v1 Vtop.
+Proof.
+  destruct v1; constructor.
+  eapply bc_of_inj_pmatch; eauto.
+Qed.
+
+Lemma bc_of_inj_args_vmatch f se1 vargs1 vargs2:
+  Val.inject_list f vargs1 vargs2 ->
+  forall v, In v vargs1 -> vmatch (bc_of_inj f se1) v Vtop.
+Proof.
+  induction 1 as [ | v1 v2 vargs1 vargs2 Hv IH]; cbn.
+  - contradiction.
+  - intros v1' [Hv1' | Hv1']; auto. subst v1'.
+    eapply bc_of_inj_vmatch; eauto.
+Qed.
+
+Lemma bc_of_inj_smatch f se1 m1 m2 b1 b2 delta:
+  Mem.inject f m1 m2 ->
+  f b1 = Some (b2, delta) ->
+  smatch (bc_of_inj f se1) m1 b1 Ptop.
+Proof.
+  intros Hm Hb.
+  split.
+  + intros chunk ofs v1 Hv1.
+    edestruct Mem.load_inject as (v2 & Hv2 & Hv); eauto.
+    eapply bc_of_inj_vmatch; eauto.
+  + intros ofs1 b1' ofs1' q i H.
+    edestruct Mem.loadbytes_inject as (bytes2 & Hbytes2 & Hv'); eauto.
+    inv Hv'. inv H4. inv H2.
+    eapply bc_of_inj_pmatch; eauto.
+Qed.
+
+Lemma bc_of_inj_mmatch f se1 m1 m2:
+  Mem.inject f m1 m2 ->
+  mmatch (bc_of_inj f se1) m1 mtop.
+Proof.
+  intros Hm. split.
+  - intros b1 Hb1. cbn in *.
+    destruct (f b1) as [[b2 delta] | ]; try discriminate.
+    destruct Genv.invert_symbol; discriminate.
+  - intros id ab b1 Hb1 H. cbn in *.
+    rewrite Maps.PTree.gempty in H. discriminate.
+  - intros b1 Hb1stk Hb1inv. cbn in *.
+    destruct (f b1) as [[b2 delta] | ] eqn:Hb; try congruence.
+    eapply bc_of_inj_smatch; eauto.
+  - intros b1 Hb1. cbn in *.
+    destruct (f b1) as [[b2 delta] | ] eqn:Hb; try congruence.
+    eapply bc_of_inj_smatch; eauto.
+  - intros b1 Hb1. cbn in *.    
+    destruct (f b1) as [[b2 delta] | ] eqn:Hb; try congruence.
+    eapply Mem.valid_block_inject_1; eauto.
+Qed.
+
+Lemma bc_of_inj_nostack f se1:
+  bc_nostack (bc_of_inj f se1).
+Proof.
+  intros b. cbn.
+  destruct f; try congruence.
+  destruct Genv.invert_symbol; congruence.
+Qed.
+
+(** * Lemmas for establish sound_state invariant using ro and injp in VA passes *)
+
+(** ** 1st step: Initialize the sound_state at query *)
+Lemma sound_memory_ro_sound_state:
+  forall j m m' se tse vargs vf vf' vargs' prog,
+    Mem.inject j m m' ->
+    Val.inject j vf vf' ->
+    Val.inject_list j vargs vargs' ->
+    Genv.match_stbls j se tse ->
+    sound_memory_ro se m ->
+    sound_state prog se (Callstate nil vf vargs m).
+Proof.
+  intros.
+  set (bc := bc_of_inj j se).
+  econstructor. instantiate (1:= bc).
+  constructor; eauto.
+  + eapply bc_of_inj_vmatch; eauto.
+  + eapply bc_of_inj_args_vmatch; eauto.
+  + red in H3. destruct H3 as [H3 H3'].
+      eapply romatch_exten; eauto.
+      intros. unfold bc, bc_of_inj, bc_of_symtbl.
+      simpl. split; intro.
+      *
+      destruct (j b) as [[b' d']|] eqn:Hf0; try congruence.
+      destruct (Genv.invert_symbol se b); try congruence.
+      *
+      destruct (Genv.invert_symbol se b) eqn:Hinv; try congruence.
+      inversion H4. subst id. inversion H2.
+      apply Genv.invert_find_symbol in Hinv. exploit mge_dom; eauto.
+      eapply Genv.genv_symb_range; eauto.
+      intros [b2 Hf0]. rewrite Hf0. reflexivity.
+    + eapply bc_of_inj_mmatch; eauto.
+    + eapply bc_of_inj_genv_match; eauto.
+    + eapply bc_of_inj_nostack; eauto.
+Qed.
+
+(** ** 2nd step *)
+
+
+
+
+
 
 (** ** Soundness of the initial memory abstraction *)
 
